split_ifs.lean
@@ -1,0 +1,103 @@
+/- Copying out split_ifs from mathlib so I can understand it. -/
+
+open expr tactic
+
+namespace tactic
+open interactive
+
+-- meta def fold_test (e : expr) : tactic unit :=
+--     trace $ expr.fold e [] (λ e n l, (e,n) :: l)
+-- constant α : Type
+-- constant f : α → α
+-- example : true := 
+-- begin
+--   (to_expr ```(λ x : α, (λ y, x) $ f $ f x) >>= fold_test)
+-- end
+
+/-- Returns the condition of a  -/
+meta def find_if_cond : expr → option expr | e := -- note the `| e` style.
+e.fold none $ λ e _ acc, acc <|> do
+    c ← match e with
+        | `(@ite %%c %%_ _ _ _) := some c
+        | `(@dite %%c %%_ _ _ _) := some c
+        | _ := none
+        end,
+    guard ¬c.has_var,
+    find_if_cond c <|> -- Why does this need to be recursive?
+    return c 
+
+/-- Find an if condition at one of the locations. -/
+meta def find_if_cond_at (at_ : loc) : tactic (option expr) := do
+lctx ← at_.get_locals, -- get the local context
+lctx ← lctx.mmap infer_type, --get the types
+tgt ← target,
+let es := if at_.include_goal then tgt::lctx else lctx,
+pure $ find_if_cond $ es.foldr app (default expr) -- jam all of the terms into one giant expression and run find_if_cond on it.
+
+-- make a new simp attribute called "split_if_reduction"
+run_cmd mk_simp_attr `split_if_reduction
+-- Add "split_if_reduction" attributes to these if-reductions
+attribute [split_if_reduction] if_pos if_neg dif_pos dif_neg
+
+meta def reduce_ifs_at (at_ : loc) : tactic unit := do
+sls ← get_user_simp_lemmas `split_if_reduction,
+let cfg : simp_config := { fail_if_unchanged := ff },
+let discharger := assumption <|> (applyc `not_not_intro >> assumption),
+hs ← at_.get_locals, 
+hs.mmap' (λ h, simp_hyp sls [] h cfg discharger >> skip),
+when at_.include_goal (simp_target sls [] cfg discharger)
+
+/-- Perform an if-split with the condition `c`, give the new hypothesis the name `n`. -/
+meta def split_if1 (c : expr) (n : name) (at_ : loc) : tactic unit := 
+by_cases c n *> reduce_ifs_at at_
+
+/--Pull a name from a ref list and use that, otherwise get a boring fresh name. -/
+private meta def get_next_name (names : ref (list name)) : tactic name := do
+ns ← read_ref names,
+match ns with
+| [] := get_unused_name `h
+| (n::ns) := do write_ref names ns, return n 
+end
+
+/-- Check that the given condition isn't already in the local context. -/
+private meta def value_known (c : expr) : tactic bool :=
+(find_assumption c $> tt)
+<|> (find_assumption `(¬%%c) $> tt)
+<|> (pure ff)
+
+private meta def split_ifs_core (at_: loc) (names : ref (list name)) : list expr → tactic unit := λ done, do
+some cond ← find_if_cond_at at_ | fail "no ite or dite expressions found",
+let cond := match cond with `(¬%%p) := p | p := p end, -- strip off the ¬
+if cond ∈ done then skip else do -- skip conditions which have already been done.
+no_split ← value_known cond,
+if no_split then do
+    reduce_ifs_at at_,
+    try (split_ifs_core (cond :: done)) 
+else do
+    n ← get_next_name names, -- pull a new name off the shelf.
+    split_if1 cond n at_,
+    try (split_ifs_core (cond :: done))
+
+meta def split_ifs (names : list name) (at_ : loc := loc.ns [none]) /-by default do the target.-/ :=
+using_new_ref names $ λ names, split_ifs_core at_ names []
+
+namespace interactive
+open interactive.types
+/-- Splits all if-then-else-expressions into multiple goals.
+
+Given a goal of the form `g (if p then x else y)`, `split_ifs` will produce
+two goals: `p ⊢ g x` and `¬p ⊢ g y`.
+
+If there are multiple ite-expressions, then `split_ifs` will split them all,
+starting with a top-most one whose condition does not contain another
+ite-expression.
+
+`split_ifs at *` splits all ite-expressions in all hypotheses as well as the goal.
+
+`split_ifs with h₁ h₂ h₃` overrides the default names for the hypotheses.
+-/
+meta def split_ifs (at_ : parse location) (names : parse with_ident_list) : tactic unit :=
+tactic.split_ifs names at_
+
+end interactive
+end tactic
