docs/meta_2.md
@@ -9,6 +9,19 @@
 - `mk_id_proof`
 
 [TODO] from `simp_tactic.lean`
-- `dunfold` vs `dsimp` vs `delta`.
+- `dunfold` vs `dsimp` vs `delta`? 
+- What do `pre` and `post` do in `dsimp`?
+- What is a discharger?
+- What do all of the options in `simp_config` do?
+- `simp`, what does it mean to dicharge? what exactly are simp lemmas? What are 
+- Simp attributes minutiae such as `mk_simp_attr`
 
 [TODO] `constructor_tactic.lean`.
+
+[TODO] `init/meta/ref.lean`
+
+[TODO] `%` antiquotation.
+
+# interactive
+
+- `loc` is either a 'wildcard', which means "everywhere", or a list of `option name`s. `none` means `target` and `some n` means `n` in the local context.
